enums and closed sums

tests/layeff/LowParseWriters.Compat.fst
@@ -55,3 +55,86 @@ let parse_vllist_correct
 let parse_vlbytes_correct
   min max
 = ()
+
+let parse_enum
+  #key p e
+=
+  make_parser
+    (LP.parse_enum_key (get_parser p) e)
+    (LP.serialize_enum_key _ (get_serializer p) e)
+    (LP.jump_enum_key (dsnd p).jumper e)
+
+let rec glb_list_of_strong
+  (#t: eqtype)
+  (f: (t -> Tot LP.parser_kind))
+  (l: list t)
+  (f_strong: ((x: t) -> Lemma (List.Tot.mem x l ==> (f x).LP.parser_kind_subkind == Some LP.ParserStrong)))
+: Lemma
+  (requires (Cons? l))
+  (ensures ((LP.glb_list_of f l).LP.parser_kind_subkind == Some LP.ParserStrong))
+= match l with
+  | [a] ->
+    f_strong a
+  | a :: q ->
+    f_strong a;
+    glb_list_of_strong f q f_strong
+
+let weaken_parse_cases_kind_strong_parser_kind
+  (s: LP.sum { Cons? (LP.Sum?.e s) })
+  (f: (x: LP.sum_key s) -> Tot (k: LP.parser_kind & LP.parser k (LP.sum_type_of_tag s x)))
+  (f_strong: (x: LP.sum_key s) -> Lemma ((dfst (f x)).LP.parser_kind_subkind == Some LP.ParserStrong))
+: Lemma
+  ((LP.weaken_parse_cases_kind s f).LP.parser_kind_subkind == Some LP.ParserStrong)
+=
+  let keys : list (LP.sum_key_type s) = List.Tot.map fst (LP.sum_enum s) in
+  glb_list_of_strong #(LP.sum_key_type s) (fun (x: LP.sum_key_type s) ->
+    if List.Tot.mem x keys
+    then let (| k, _ |) = f x in k
+    else LP.default_parser_kind
+  ) (List.Tot.map fst (LP.sum_enum s))
+  (fun x ->
+    if List.Tot.mem x keys
+    then f_strong x
+    else ()
+  )
+
+let parse_sum_kind_strong
+  (ps: parse_sum_t)
+: Lemma
+  ((LP.parse_sum_kind ps.sum_kt ps.sum_t ps.sum_pc).LP.parser_kind_subkind == Some LP.ParserStrong)
+= weaken_parse_cases_kind_strong_parser_kind ps.sum_t ps.sum_pc (fun x -> let p = ps.sum_pc' x in ())
+  
+let parse_sum
+  ps
+=
+  [@inline_let]
+  let _ = parse_sum_kind_strong ps in
+  make_parser
+    (LP.parse_sum ps.sum_t ps.sum_p ps.sum_pc)
+    (LP.serialize_sum #ps.sum_kt ps.sum_t #ps.sum_p ps.sum_s #ps.sum_pc ps.sum_sc)
+    (LP.jump_sum ps.sum_t (dsnd (ps.sum_p')).jumper ps.sum_r ps.sum_pc (fun x -> (dsnd (ps.sum_pc' x)).jumper) ps.sum_destr)
+
+let valid_synth_parse_sum
+  ps k
+= {
+  valid_synth_valid = (fun h b pos pos' ->
+    let sl = LP.make_slice b (B.len b) in
+    assert (LP.valid (LP.parse_enum_key ps.sum_p (LP.sum_enum ps.sum_t) `LP.nondep_then` dsnd (ps.sum_pc k)) h sl pos);
+    let (k', _) = LP.contents (LP.parse_enum_key ps.sum_p (LP.sum_enum ps.sum_t) `LP.nondep_then` dsnd (ps.sum_pc k)) h sl pos in
+    assert (k' == k);
+    LP.valid_nondep_then h (LP.parse_enum_key ps.sum_p (LP.sum_enum ps.sum_t)) (dsnd (ps.sum_pc k)) sl pos;
+    assert (LP.valid (LP.parse_enum_key ps.sum_p (LP.sum_enum ps.sum_t)) h sl pos);
+    assert (LP.contents (LP.parse_enum_key ps.sum_p (LP.sum_enum ps.sum_t)) h sl pos == k);
+    LP.valid_sum_intro h ps.sum_t ps.sum_p ps.sum_pc sl pos
+  );
+  valid_synth_size = (fun x ->
+    let (k', pl) = LP.coerce (dfst (parse_enum ps.sum_p' (LP.sum_enum ps.sum_t)) & dfst (ps.sum_pc' k)) (x <: (dfst (parse_enum ps.sum_p' (LP.sum_enum ps.sum_t) `star` ps.sum_pc' k))) in
+    let y = LP.synth_sum_case ps.sum_t k pl in
+    assert (LP.sum_tag_of_data ps.sum_t y == k);
+    LP.synth_sum_case_inverse ps.sum_t k;
+    LP.synth_sum_case_injective ps.sum_t k;
+    LP.synth_injective_synth_inverse_synth_inverse_recip (LP.synth_sum_case ps.sum_t k) (LP.synth_sum_case_recip ps.sum_t k) ();
+    assert (LP.synth_sum_case_recip ps.sum_t k y == pl);
+    LP.serialize_sum_eq ps.sum_t ps.sum_s #ps.sum_pc ps.sum_sc y
+  );
+}
