tests/layeff/LowParseWriters.Compat.fsti
@@ -116,3 +116,60 @@ val parse_vlbytes_correct
     [SMTPat (get_parser (parse_vlbytes min max))];
     [SMTPat (get_serializer (parse_vlbytes min max))];
   ]]
+
+inline_for_extraction
+noextract
+noeq
+type parse_sum_t = {
+  sum_kt: LP.parser_kind;
+  sum_t: (sum_t: LP.sum {
+    Cons? (LP.sum_enum sum_t)
+  });
+  sum_p: LP.parser sum_kt (LP.sum_repr_type sum_t);
+  sum_r: LP.leaf_reader sum_p;
+  sum_s: LP.serializer sum_p;
+  sum_pc: ((x: LP.sum_key sum_t) -> Tot (k: LP.parser_kind & LP.parser k (LP.sum_type_of_tag sum_t x)));
+  sum_sc: ((x: LP.sum_key sum_t) -> Tot (LP.serializer (dsnd (sum_pc x))));
+  sum_destr: LP.dep_maybe_enum_destr_t (LP.sum_enum sum_t) (LP.jump_sum_aux_payload_t sum_t sum_pc);
+  sum_p' : (p' : parser {
+    dfst p' == LP.sum_repr_type sum_t /\
+    get_parser_kind p' == sum_kt /\
+    get_parser p' == sum_p /\
+    get_serializer p' == sum_s
+  });
+  sum_pc' : ((x: LP.sum_key sum_t) -> Tot (p': parser {
+    dfst p' == LP.sum_type_of_tag sum_t x /\
+    get_parser_kind p' == dfst (sum_pc x) /\
+    get_parser p' == LP.coerce (LP.parser (get_parser_kind p') (dfst p')) (dsnd (sum_pc x)) /\
+    get_serializer p' == LP.coerce (LP.serializer (get_parser p')) (sum_sc x)
+  }));
+}
+
+inline_for_extraction
+noextract
+val parse_enum
+  (#key: eqtype)
+  (p: parser { hasEq (dfst p) })
+  (e: LP.enum key (dfst p))
+: Tot (p': parser {
+    dfst p' == LP.enum_key e /\
+    get_parser_kind p' == LP.parse_filter_kind (get_parser_kind p) /\
+    get_parser p' == LP.parse_enum_key (get_parser p) e /\
+    get_serializer p' == LP.serialize_enum_key _ (get_serializer p) e
+  })
+
+inline_for_extraction
+noextract
+val parse_sum
+  (ps: parse_sum_t)
+: Tot (q: parser {
+    dfst q == LP.sum_type ps.sum_t /\
+    get_parser_kind q == LP.parse_sum_kind ps.sum_kt ps.sum_t ps.sum_pc /\
+    get_parser q == LP.parse_sum ps.sum_t ps.sum_p ps.sum_pc /\
+    get_serializer q == LP.serialize_sum #ps.sum_kt ps.sum_t #ps.sum_p ps.sum_s #ps.sum_pc ps.sum_sc
+  })
+
+val valid_synth_parse_sum
+  (ps: parse_sum_t)
+  (k: LP.sum_key ps.sum_t)
+: Tot (valid_synth_t (parse_enum ps.sum_p' (LP.sum_enum ps.sum_t) `star` ps.sum_pc' k) (parse_sum ps) (fun (k', _) -> k' == k) (fun (_, pl) -> LP.Sum?.synth_case ps.sum_t k pl))
